compcertox/PEnv.v
@@ -1,0 +1,506 @@
+From compcert Require Import
+     AST Coqlib Maps Values Integers Errors Events
+     Globalenvs Memory Floats Join Ctypes Values Cop Clight.
+Require Import Lia.
+Require SimplLocalsproof.
+
+(** ------------------------------------------------------------------------- *)
+(** PVal and PEnv  *)
+Open Scope Z_scope.
+
+Inductive val : Type :=
+| Val : Values.val -> type -> val
+| Array : Z -> ZMap.t val -> type -> val.
+(* TODO: support struct *)
+(* | Struct : list ident -> PMap.t val -> val. *)
+
+Definition type_of_pv (pv: val) :=
+  match pv with
+  | Val _ ty | Array _ _ ty => ty
+  end.
+
+Fixpoint size_of_type (t: type): Z :=
+  match t with
+  | Tint I32 _ _ => 4
+  | Tarray t' n _ => size_of_type t' * Z.max 0 n
+  | _ => 0
+  end.
+
+Inductive init_pv: val -> Prop :=
+| init_pv_int attr:
+  init_pv (Val (Vint Int.zero) (Tint I32 Unsigned attr))
+| init_pv_array n ty_elem attr arr:
+  (forall i, 0 <= i < n -> init_pv (ZMap.get i arr)) ->
+  (forall i, 0 <= i < n -> type_of_pv (ZMap.get i arr) = ty_elem) ->
+  init_pv (Array n arr (Tarray ty_elem n attr)).
+
+Record privvar : Type :=
+  mkprivvar {
+      pvar_init:> val;
+      pvar_spec: init_pv pvar_init;
+      pvar_size: size_of_type (type_of_pv pvar_init) < Int.max_unsigned;
+    }.
+
+
+Definition penv : Type := PTree.t val.
+(** typed location: the type information is used to calculate the correct
+        offset when we establish a relation between penv and CompCert memory *)
+Inductive loc : Type := Loc: type -> list (Z * type) -> loc.
+
+(** Again, the type information is used when relate [pread] with
+    [deref_loc]. Consider this relation as a specification of the function of
+    type [val -> loc -> Values.val * type] *)
+Inductive pread_val: val -> loc -> Values.val -> type -> Prop :=
+(* TODO: be more tolerent on typing *)
+| pread_nil: forall v ty, pread_val (Val v ty) (Loc ty nil) v ty
+| pread_cons:
+  forall n arr ty ty_elem ty_v i v attr rest,
+    0 <= i < n ->
+    pread_val (ZMap.get i arr) (Loc ty_v rest) v ty_v ->
+    ty = Tarray ty_elem n attr ->
+    pread_val (Array n arr ty) (Loc ty_v ((i, ty_elem) :: rest)) v ty_v.
+
+Inductive pread: penv -> ident -> loc -> Values.val -> type -> Prop :=
+| pread_intro: forall pe id l pv v ty,
+    pe!id = Some pv ->
+    pread_val pv l v ty ->
+    pread pe id l v ty.
+
+Inductive pwrite_val: val -> loc -> Values.val -> val -> type -> Prop :=
+| pwrite_nil: forall old_v new_v ty
+                (VTY: val_casted new_v ty),
+    pwrite_val (Val old_v ty) (Loc ty nil) new_v (Val new_v ty) ty
+| pwrite_cons:
+  forall old_arr new_arr n i ty old_pv new_pv rest new_v ty_v attr ty_elem,
+    0 <= i < n ->
+    old_pv = ZMap.get i old_arr ->
+    pwrite_val old_pv (Loc ty_v rest) new_v new_pv ty_v ->
+    new_arr = ZMap.set i new_pv old_arr ->
+    ty = Tarray ty_elem n attr ->
+    pwrite_val (Array n old_arr ty) (Loc ty_v ((i, ty_elem) :: rest))
+      new_v (Array n new_arr ty) ty_v.
+
+Inductive pwrite: penv -> ident -> loc -> Values.val -> penv -> type -> Prop :=
+| pwrite_intro:  forall pe id l pe' v old_pv new_pv ty ch,
+    pe!id = Some old_pv ->
+    pwrite_val old_pv l v new_pv ty ->
+    pe' =  PTree.set id new_pv pe ->
+    access_mode ty = By_value ch ->
+    pwrite pe id l v pe' ty.
+
+
+(** ------------------------------------------------------------------------- *)
+(** The relation between persistent environment and memory *)
+
+Section WITH_CE.
+
+  Variable (ce: composite_env).
+  (** The relation between a pvalue and memory *)
+  Inductive pvalue_match: block -> Z -> val -> Mem.mem -> Prop :=
+  | pval_match:
+    forall b ofs ty chunk v m
+      (ACCESS: access_mode ty = By_value chunk)
+      (LOAD: Mem.load chunk m  b ofs = Some v)
+      (WRITABLE: Mem.valid_access m chunk b ofs Writable),
+      pvalue_match b ofs (Val v ty) m
+  | parray_match:
+    forall b ofs n parr ty m attr ty_elem
+      (TARRAY: ty = Tarray ty_elem n attr)
+      (NO_OVERFLOW: ofs + n * sizeof ce ty_elem <= Ptrofs.max_unsigned)
+      (TYPE: forall i, 0 <= i < n -> ty_elem = type_of_pv (ZMap.get i parr))
+      (MATCH: forall i, 0 <= i < n ->
+                   pvalue_match b (ofs + i * sizeof ce ty_elem) (ZMap.get i parr) m),
+      pvalue_match b ofs (Array n parr ty) m.
+
+  (** The relation between the penv and memory *)
+  Inductive penv_match: Genv.symtbl -> (penv * Mem.mem) -> Mem.mem -> Prop :=
+  | penv_match_intro:
+    forall se pe m tm mpersistent
+      (MJOIN: join mpersistent m tm)
+      (MVALUE: forall id v, PTree.get id pe = Some v ->
+                       exists b, Genv.find_symbol se id = Some b /\
+                              pvalue_match b 0 v mpersistent),
+      penv_match se (pe, m) tm.
+
+  Lemma size_type_chunk ty ch:
+    access_mode ty = By_value ch ->
+    size_chunk ch = sizeof ce ty.
+  Proof.
+    intros. destruct ty; inv H; cbn in *; try easy.
+    - destruct i; destruct s; inv H1; easy.
+    - destruct f; inv H1; easy.
+  Qed.
+
+  Lemma pvalue_match_unchanged:
+    forall P ma mb b ofs pv,
+      pvalue_match b ofs pv ma ->
+      Mem.unchanged_on P ma mb ->
+      (forall i, ofs <= i < ofs + sizeof ce (type_of_pv pv) -> P b i) ->
+      pvalue_match b ofs pv mb.
+  Proof.
+    intros * H HM HP. induction H.
+    - cbn in *. erewrite <- size_type_chunk in HP; eauto.
+      eapply pval_match; eauto.
+      + exploit Mem.load_unchanged_on; eauto.
+      + destruct WRITABLE as [A B].
+        split; eauto.
+        intros x Hx. specialize (A _ Hx).
+        eapply Mem.perm_unchanged_on; eauto.
+    - eapply parray_match; eauto.
+      intros i Hi. apply H; eauto.
+      intros x Hx. apply HP.
+      subst. cbn.
+      clear - Hi Hx TYPE. rewrite Z.max_r. 2: lia.
+      specialize (TYPE _ Hi). subst.
+      pose proof (sizeof_pos ce (type_of_pv (ZMap.get i parr))).
+      revert H Hx. generalize (sizeof ce (type_of_pv (ZMap.get i parr))).
+      intros z Hp Hz. split.
+      + transitivity (ofs + i * z). 2: apply Hz.
+        cut (0 <= i * z). lia. apply Z.mul_nonneg_nonneg; lia.
+      + eapply Z.lt_le_trans. apply Hz.
+        rewrite <- Z.add_assoc.
+        apply Z.add_le_mono_l.
+        cut (i + 1 <= n). 2: lia. intros Ha.
+        transitivity (z * (i + 1)). lia.
+        apply Z.mul_le_mono_nonneg_l; lia.
+  Qed.
+
+  Lemma pvalue_match_join:
+    forall ma mb m b ofs pv,
+      pvalue_match b ofs pv mb ->
+      join ma mb m ->
+      pvalue_match b ofs pv m.
+  Proof.
+    intros * H HJ. induction H.
+    - eapply pval_match; eauto.
+      + exploit load_join. apply HJ. rewrite LOAD.
+        intros HO. inv HO. reflexivity.
+      + destruct WRITABLE as [A B]. split; eauto.
+        intros x Hx. specialize (A _ Hx).
+        eapply perm_join; eauto.
+    - eapply parray_match; eauto.
+  Qed.
+
+  (** The relation between location and pointer offset *)
+  Inductive match_loc: loc -> Z -> Prop :=
+  | match_base:
+    forall ty, match_loc (Loc ty nil) 0
+  | match_index:
+    forall i rest ofs_start ofs_elem ty ty_v
+      (BASE: match_loc (Loc ty_v rest) ofs_start)
+      (OFS: ofs_elem = i * sizeof ce ty)
+      (NO_OVERLAP: ofs_start + sizeof ce ty_v <= sizeof ce ty)
+      (POS: i >= 0),
+      match_loc (Loc ty_v ((i, ty) :: rest)) (ofs_start + ofs_elem).
+
+  Lemma int_max_le_ptrofs_max: Int.modulus - 1 <= Ptrofs.max_unsigned.
+  Proof.
+    unfold Int.modulus, Ptrofs.max_unsigned, Ptrofs.modulus.
+    assert (Int.wordsize <= Ptrofs.wordsize)%nat.
+    unfold Ptrofs.wordsize, Int.wordsize, Wordsize_32.wordsize, Wordsize_Ptrofs.wordsize.
+    destruct Archi.ptr64; lia.
+    assert (two_power_nat Int.wordsize <= two_power_nat Ptrofs.wordsize).
+    {
+      rewrite !two_power_nat_two_p.
+      apply two_p_monotone. extlia.
+    }
+    lia.
+  Qed.
+
+  Lemma match_loc_app:
+    forall l ofs_start i ty ofs_elem ty_prev n attr,
+      match_loc (Loc ty_prev l) ofs_start ->
+      ofs_elem = i * sizeof ce ty ->
+      ty_prev = Tarray ty n attr ->
+      0 <= i < n ->
+      match_loc (Loc ty (l ++ (i, ty) :: nil)) (ofs_start + ofs_elem).
+  Proof.
+    intros l. induction l.
+    - intros * A B C D.
+      inv A. cbn.
+      replace (i * sizeof ce ty) with (0 + i * sizeof ce ty) by reflexivity.
+      constructor; eauto. constructor. reflexivity. lia.
+    - intros * A B C D. inv A. rewrite <- app_comm_cons.
+      replace (ofs_start0 + i0 * sizeof ce ty0 + i * sizeof ce ty)
+        with (ofs_start0 + i * sizeof ce ty + i0 * sizeof ce ty0)
+        by lia.
+      constructor; eauto.
+      cbn in *. revert NO_OVERLAP.
+      generalize (sizeof_pos ce ty).
+      generalize (sizeof ce ty). intros z A B.
+      transitivity (ofs_start0 + z * Z.max 0 n); eauto.
+      rewrite <- Z.add_assoc.
+      apply Z.add_le_mono_l.
+      rewrite Z.max_r by lia.
+      transitivity (z * (i + 1)); try lia.
+      apply Z.mul_le_mono_nonneg_l; lia.
+  Qed.
+
+  (** Correctness of [pread] and [pwrite] *)
+
+  (** This lemma represents the following diagram
+    pv ---- loc ---->  v
+    |                  |
+  match                =
+    |                  |
+    m --- (b, ofs) --> v *)
+  Lemma pread_val_correct':
+    forall pv l ty ofs v tm base b,
+      pread_val pv l v ty ->
+      match_loc l ofs ->
+      pvalue_match b base pv tm ->
+      base + ofs <= Ptrofs.max_unsigned ->
+      base >= 0 ->
+      deref_loc ty tm b (Ptrofs.repr (ofs + base)) Full v.
+  Proof.
+    intros until b. intros H.
+    revert base ofs.
+    induction H.
+    - intros. inv H. inv H0.
+      eapply deref_loc_value; eauto.
+      cbn.
+      rewrite Ptrofs.unsigned_repr; eauto. lia.
+    - intros. inv H2. inv H3. inv TARRAY.
+      rewrite <- Z.add_assoc.
+      apply IHpread_val; eauto.
+      rewrite Z.add_comm. eauto.
+      lia.
+      apply Z.le_ge.
+      apply Z.add_nonneg_nonneg; try lia.
+      apply Z.mul_nonneg_nonneg; try lia.
+      pose proof (sizeof_pos ce ty_elem0). lia.
+  Qed.
+
+  Lemma pread_val_correct:
+    forall pv l ty ofs v tm b,
+      pread_val pv l v ty ->
+      match_loc l ofs ->
+      pvalue_match b 0 pv tm ->
+      ofs <= Ptrofs.max_unsigned ->
+      deref_loc ty tm b (Ptrofs.repr ofs) Full v.
+  Proof.
+    intros. exploit pread_val_correct'; eauto.
+    lia. rewrite Z.add_0_r. easy.
+  Qed.
+
+  Lemma pwrite_val_type_of_pv:
+    forall pv l v pv' ty,
+      pwrite_val pv l v pv' ty ->
+      type_of_pv pv = type_of_pv pv'.
+  Proof. intros * H. induction H; eauto. Qed.
+
+  Lemma match_loc_pos:
+    forall l ofs, match_loc l ofs -> ofs >= 0.
+  Proof.
+    intros * A. induction A. lia.
+    subst.
+    apply Z.le_ge.
+    apply Z.add_nonneg_nonneg; try lia.
+    apply Z.mul_nonneg_nonneg; try lia.
+    pose proof (sizeof_pos ce ty). lia.
+  Qed.
+
+  (** This lemma represents the following diagram
+    pv ---- loc ---->  pv'
+    |                  |
+  match                match
+    |                  |
+    m --- (b, ofs) --> m' *)
+  Lemma pwrite_val_correct':
+    forall pv pv' ch l ty base ofs v tm b,
+      pwrite_val pv l v pv' ty ->
+      match_loc l ofs ->
+      pvalue_match b base pv tm ->
+      access_mode ty = By_value ch ->
+      exists tm', Mem.store ch tm b (base + ofs) v = Some tm'
+             /\ pvalue_match b base pv' tm'.
+  Proof.
+    intros until b. intros H. revert ofs base.
+    induction H.
+    - intros. inv H. inv H0. rewrite H1 in ACCESS. inv ACCESS.
+      rewrite Z.add_0_r.
+      edestruct Mem.valid_access_store as (tm' & Hm). eauto.
+      exists tm'. split; eauto. econstructor; eauto.
+      + erewrite Mem.load_store_same; eauto. f_equal.
+        eapply SimplLocalsproof.val_casted_load_result; eauto.
+      + eapply Mem.store_valid_access_1; eauto.
+    - intros.
+      inv H4. inv H5. inv TARRAY.
+      exploit MATCH; eauto. intros.
+      edestruct IHpwrite_val as (tm' & A & B); eauto.
+      exists tm'. split.
+      + rewrite <- A. f_equal. rewrite <- Z.add_assoc. f_equal. lia.
+      + econstructor; eauto.
+        * intros ix Hix. destruct (zeq i ix).
+          -- subst. rewrite ZMap.gss.
+             erewrite <- pwrite_val_type_of_pv; eauto.
+          -- rewrite ZMap.gso by congruence.
+             specialize (TYPE _ Hix). eauto.
+        * intros ix Hix. destruct (zeq i ix).
+          -- subst. rewrite ZMap.gss. apply B.
+          -- rewrite ZMap.gso by congruence.
+             specialize (MATCH _ Hix).
+             specialize (TYPE _ Hix). subst.
+             remember (sizeof ce (type_of_pv (ZMap.get ix old_arr)))
+               as elem_sz eqn: Hsz.
+             eapply pvalue_match_unchanged; eauto.
+             instantiate
+               (1 := fun (_: block) (ofsx: Z) =>
+                       ofsx < base + i * elem_sz + ofs_start
+                       \/ ofsx >= base + i * elem_sz + ofs_start + size_chunk ch
+               ).
+             eapply Mem.store_unchanged_on; eauto.
+             intros z Hz. lia.
+             cbn. intros z Hz. rewrite <- Hsz in Hz.
+             assert (ofs_start + size_chunk ch <= elem_sz).
+             { erewrite size_type_chunk; eauto. }
+             cut (i < ix \/ i > ix). 2: lia.
+             intros [C | C].
+             ++ right.
+                cut (z >= base + (i+1) * elem_sz); try lia.
+                cut (ix * elem_sz >= (i + 1) * elem_sz); try lia.
+                apply Zmult_ge_compat_r; lia.
+             ++ left.
+                cut (ofs_start >= 0).
+                cut (ix * elem_sz + elem_sz <= i * elem_sz). lia.
+                rewrite Zmult_succ_l_reverse.
+                apply Zmult_le_compat_r; lia.
+                eapply match_loc_pos. eauto.
+  Qed.
+
+  Lemma pwrite_val_correct:
+    forall pv pv' ch l ty ofs v tm b,
+      pwrite_val pv l v pv' ty ->
+      match_loc l ofs ->
+      pvalue_match b 0 pv tm ->
+      access_mode ty = By_value ch ->
+      exists tm', Mem.store ch tm b ofs v = Some tm'
+             /\ pvalue_match b 0 pv' tm'.
+  Proof. intros. exploit pwrite_val_correct'; eauto. Qed.
+
+End WITH_CE.
+
+Program Definition empty_fragment (b: block) (lo hi: Z) :=
+  {|
+    Mem.mem_contents := PMap.init (ZMap.init Undef);
+    Mem.mem_access :=
+      PMap.set b
+        (fun ofs k => if zle lo ofs && zlt ofs hi then Some Writable else None)
+        (PMap.init (fun ofs k => None));
+    Mem.nextblock := Pos.succ b;
+    Mem.alloc_flag := false;
+  |}.
+Next Obligation. Admitted.
+Next Obligation. Admitted.
+
+Definition init_fragment' (b: block) (sz: Z) :=
+  match store_zeros (empty_fragment b 0 sz) b 0 sz with
+  | Some m => m
+  | None => Mem.empty
+  end.
+
+Definition init_fragment (id: ident) (pv: val) (se: Genv.symtbl) :=
+  match Genv.find_symbol se id with
+  | Some b => init_fragment' b (size_of_type (type_of_pv pv))
+  | None => Mem.empty
+  end.
+
+Lemma read_as_zero_weaken m b ofs ofs' len len':
+  ofs' >= ofs -> ofs' + len' <= ofs + len ->
+  Genv.read_as_zero m b ofs len ->
+  Genv.read_as_zero m b ofs' len'.
+Proof.
+  unfold Genv.read_as_zero. intros. apply H1; eauto; lia.
+Qed.
+
+Lemma init_pv_size ce pv ty:
+  init_pv pv ->
+  ty = type_of_pv pv ->
+  size_of_type ty = sizeof ce ty.
+Admitted.
+
+Lemma init_pvalue_match ce b pv:
+  init_pv pv ->
+  pvalue_match ce b 0 pv (init_fragment' b (size_of_type (type_of_pv pv))).
+Proof.
+  intros H. unfold init_fragment'.
+  remember (size_of_type (type_of_pv pv)) as sz.
+  assert (exists m, store_zeros (empty_fragment b 0 sz) b 0 sz = Some m)
+    as (m & Hm).
+  {
+    eapply Genv.store_zeros_exists.
+    admit.
+  }
+  rewrite Hm.
+  assert (Hp: Mem.range_perm m b 0 (0 + sz) Cur Writable).
+  {
+    admit.
+  }
+  eapply Genv.store_zeros_read_as_zero in Hm.
+  assert (H0: (4 | 0)). apply Z.divide_0_r.
+  revert Hm. revert sz Heqsz H0 Hp. generalize 0.
+  induction H; cbn; intros ofs sz Hsz Hdiv Hp Hread.
+  - subst. econstructor. reflexivity.
+    + specialize (Hread Mint32 ofs).
+      exploit Hread; cbn; eauto; try lia.
+    + split; eauto.
+  - econstructor; eauto.
+    + admit.
+    + intros i Hi. specialize (H1 i Hi). eauto.
+    + intros i Hi. specialize (H0 i Hi).
+      eapply H0. reflexivity.
+      * admit.
+      * admit.
+      * rewrite H1; eauto.
+        assert (sizeof ce ty_elem >= 0).
+        { apply sizeof_pos. }
+        eapply read_as_zero_weaken. 3: eauto.
+        -- lia.
+        -- rewrite <- Z.add_assoc. apply Z.add_le_mono_l.
+           rewrite Z.add_comm.
+           assert (Hs: size_of_type ty_elem = sizeof ce ty_elem).
+           admit.
+           rewrite <- Hs. subst. remember (size_of_type ty_elem) as a.
+           transitivity (a * (i + 1)). lia.
+           apply Z.mul_le_mono_nonneg_l; lia.
+Admitted.
+
+Fixpoint p0  (xs: list (ident * val)) : penv :=
+  match xs with
+  | nil => @PTree.empty val
+  | ((id, pv) :: rest) => PTree.set id pv (p0 rest)
+  end.
+
+Fixpoint m0 (xs: list (ident * val)) (se: Genv.symtbl) : mem :=
+  match xs with
+  | nil => Mem.empty
+  | ((id, ty) :: rest) => mem_combine (init_fragment id ty se) (m0 rest se)
+  end.
+
+(* Definition vars_of_program (p: program) : list (ident * val) := *)
+
+Inductive penv_mem_match ce: Genv.symtbl -> penv -> Mem.mem -> Prop :=
+| penv_mem_match_intro se pe m
+    (MPE: forall id v, PTree.get id pe = Some v ->
+          exists b, Genv.find_symbol se id = Some b /\
+          pvalue_match ce b 0 v m):
+  penv_mem_match ce se pe m.
+
+Fixpoint init_of_pvars (vs: list (ident * privvar)) : list (ident * val) :=
+  match vs with
+  | nil => nil
+  | (id, v) :: rest => (id, pvar_init v) :: (init_of_pvars rest)
+  end.
+
+Lemma vars_init ce pvars se:
+  penv_mem_match ce se
+    (p0 (init_of_pvars pvars))
+    (m0 (init_of_pvars pvars) se).
+Admitted.
+
+Variable vars_disjoint: list (ident * val) -> list (ident * val) -> Prop.
+Lemma disjoint_init_mem:
+  forall se vars1 vars2,
+    vars_disjoint vars1 vars2 ->
+    join (m0 vars1 se) (m0 vars2 se) (m0 (vars1 ++ vars2) se).
+Admitted.
